pulse/src/checker/Pulse.Checker.Comp.fst
@@ -47,7 +47,7 @@ let check (g:env)
           let px = v_as_nv x in
           assume (~(x `Set.mem` freevars (comp_post c)));
           let gx = push_binding g x (fst px) st.res in
-          let (| ty, post_typing |) = core_compute_tot_term_type gx (open_term_nv (comp_post c) px) in
+          let ty = core_compute_tot_term_type gx (open_term_nv (comp_post c) px) in
           if not (eq_tm ty tm_slprop)
           then fail g None
                  (Printf.sprintf "check_comp: ill-typed postcondition %s" (P.term_to_string (comp_post c)))
@@ -63,14 +63,14 @@ let check (g:env)
       ()
     | C_STAtomic i obs st -> 
       let stc = check_st_comp st in
-      let (| ty, i_typing |) = core_compute_tot_term_type g i in
+      let ty = core_compute_tot_term_type g i in
       if not (eq_tm ty tm_inames)
       then fail g None
              (Printf.sprintf "check_comp (atomic): type of inames term %s is %s, expected %s"
                 (P.term_to_string i) (P.term_to_string ty) (P.term_to_string tm_inames))
       else ()
     | C_STGhost i st ->
-      let (| ty, i_typing |) = core_compute_tot_term_type g i in
+      let ty = core_compute_tot_term_type g i in
       if not (eq_tm ty tm_inames)
       then fail g None
              (Printf.sprintf "check_comp (ghost): type of inames term %s is %s, expected %s"
