pulse/src/checker/Pulse.Checker.If.fst
@@ -57,7 +57,7 @@ let check
   
   let g = Pulse.Typing.Env.push_context g "check_if" e1.range in
 
-  let (| b, b_typing |) =
+  let b =
     check_tot_term g b tm_bool in
 
   let hyp = fresh g in
