pulse/src/checker/Pulse.Checker.Return.fst
@@ -27,29 +27,35 @@ module Metatheory = Pulse.Typing.Metatheory
 module RU = Pulse.RuntimeUtils
 
 let check_effect
-    (#g:env) (#e:term) (#eff:T.tot_or_ghost) (#t:term)
-    (d:typing g e eff t)
+    (g:env) (e:term) (eff:T.tot_or_ghost)
     (c:option ctag)
-: T.Tac (c:ctag & e:term & typing g e (eff_of_ctag c) t)
+: T.Tac (c:ctag & e:term)
 = match c, eff with
   | None, T.E_Total -> 
-    (| STT_Atomic, e, d |)
+    (| STT_Atomic, e |)
   | None, T.E_Ghost -> 
-    (| STT_Ghost, e, d |)
+    (| STT_Ghost, e |)
   | Some STT_Ghost, T.E_Total ->
-    (| STT_Atomic, e, d |)
+    (| STT_Atomic, e |)
   | Some STT_Ghost, T.E_Ghost -> 
-    (| STT_Ghost, e, d |)
+    (| STT_Ghost, e |)
   | _, T.E_Total -> 
-    (| STT_Atomic, e, d |)
+    (| STT_Atomic, e |)
   | _ -> 
     fail g (Some (RU.range_of_term e)) "Expected a total term, but this term has Ghost effect"
  
 
 let check_tot_or_ghost_term (g:env) (e:term) (t:term) (c:option ctag)
-: T.Tac (c:ctag & e:term & typing g e (eff_of_ctag c) t)
-= let (| e, eff, d |) = check_term_at_type g e t in
-  check_effect d c
+: T.Tac (c:ctag & e:term)
+= let (| e, eff |) = check_term_at_type g e t in
+  match c, eff with
+  | None, T.E_Total
+  | Some STT_Ghost, T.E_Total
+  | _, T.E_Total -> (| STT_Atomic, e |)
+  | None, T.E_Ghost
+  | Some STT_Ghost, T.E_Ghost -> (| STT_Ghost, e |)
+  | _ ->
+    fail g (Some (RU.range_of_term e)) "Expected a total term, but this term has Ghost effect"
   
 noeq
 type result_of_typing (g:env) =
@@ -65,9 +71,9 @@ type result_of_typing (g:env) =
 let compute_tot_or_ghost_term_type_and_u (g:env) (e:term) (c:option ctag)
 : T.Tac (result_of_typing g)
 = RU.with_error_bound (RU.range_of_term e) fun () -> // stopgap, ideally remove
-  let (| t, eff, ty, u, d |) = compute_term_type_and_u g e in
-  let (| c, e, d |) = check_effect d c in
-  R c e u ty () d
+  let (| t, eff, ty, u |) = compute_term_type_and_u g e in
+  let (| c, e |) = check_effect g t eff c in
+  R c e u ty () ()
 
 #push-options "--z3rlimit_factor 16 --fuel 0 --ifuel 1 --split_queries no"
 #restart-solver
@@ -84,12 +90,12 @@ let check_core
   let g = push_context "check_return" st.range g in
   let Tm_Return {expected_type; insert_eq=use_eq; term=t} = st.term in
   let return_type
-    : option (ty:term & u:universe & universe_of g ty u) =
+    : option (ty:term & u:universe) =
     match post_hint with
     | PostHint post ->
       assert (g `env_extends` post.g);
-      let ty_typing : universe_of g post.ret_ty post.u = () in
-      Some (| post.ret_ty, post.u, ty_typing |)
+
+      Some (| post.ret_ty, post.u |)
     | _ ->
       match inspect_term expected_type with
       | Tm_Unknown -> (
@@ -98,24 +104,24 @@ let check_core
         | TypeHint expected_type -> 
           let ty, _ = Pulse.Checker.Pure.instantiate_term_implicits g expected_type None false in
           let u = check_universe g ty in
-          Some (| ty, u, () |)
+          Some (| ty, u |)
       )
       | _ ->
         let ty, _ = Pulse.Checker.Pure.instantiate_term_implicits g expected_type None false in
         let u = check_universe g ty in
-        Some (| ty, u, () |)
+        Some (| ty, u |)
   in
   let R c t u ty uty d : result_of_typing g =
     match return_type with
     | None ->
       compute_tot_or_ghost_term_type_and_u g t ctag_ctxt
-    | Some (| ret_ty, u, ty_typing |) ->
-      let (| c, t, d |) = check_tot_or_ghost_term g t ret_ty ctag_ctxt in
-      R c t u ret_ty ty_typing d
+    | Some (| ret_ty, u |) ->
+      let (| c, t |) = check_tot_or_ghost_term g t ret_ty ctag_ctxt in
+      R c t u ret_ty () ()
   in
   let x = fresh g in
   let px = res_ppname, x in
-  let (| post_opened, post_typing |) : t:term & tot_typing (push_binding g x (fst px) ty)  t tm_slprop =
+  let post_opened : term =
       match post_hint with
       | PostHint post ->
         // we already checked for the return type
@@ -126,10 +132,10 @@ let check_core
                  please file a bug report")
         else 
          let ty_rec = post_hint_typing g post x in
-         (| open_term_nv post.post px, ty_rec.post_typing |)
+         open_term_nv post.post px
       | _ ->
-        let (| t, ty |) = check_tot_term (push_binding g x (fst px) ty) tm_emp tm_slprop in
-        (| t, ty |)    
+        let t = check_tot_term (push_binding g x (fst px) ty) tm_emp tm_slprop in
+        t
   in
   //if we're inferring a postcondition, then add an equality (if it is non-trivial)
   let use_eq = use_eq || (not (PostHint? post_hint) && not (T.term_eq ty (`unit))) in
